\documentclass{article}
\usepackage{fancyhdr}
\usepackage{lipsum}  
\usepackage{listings} 
\usepackage{xcolor}   
\usepackage{amsmath}
\usepackage{enumitem}
\usepackage{graphicx}
\usepackage{caption}
\usepackage{verbatim}

% Define macros for title and author
\newcommand{\thetitle}{STAT 641 \\ Homework 1}
\newcommand{\theauthor}{Keegan Smith}

\title{\thetitle}
\author{\theauthor}

\pagestyle{fancy}
\fancyhf{}  % Clear all header and footer fields
\fancyhead[L]{\nouppercase{\rightmark}}
\fancyhead[C]{\thetitle}  % Title in the center
\fancyhead[R]{\theauthor}  % Your name on the right

\lstset{ %
  backgroundcolor=\color{lightgray},   % choose the background color
  basicstyle=\ttfamily\small,          % size of fonts used for the code
  keywordstyle=\color{blue},           % color for keywords
  commentstyle=\color{green},          % color for comments
  stringstyle=\color{red},             % color for strings
  numbers=left,                        % where to put the line-numbers
  numberstyle=\tiny\color{gray},       % style for line-numbers
  stepnumber=1,                        % the step between two line-numbers
  numbersep=5pt,                       % how far the line-numbers are from the code
  frame=single,                        % adds a frame around the code
  rulecolor=\color{black},             % frame color
  breaklines=true,                     % automatic line breaking
  breakatwhitespace=false,             % automatic breaks should only happen at whitespace
  showspaces=false,                    % don't show spaces in the code
  showstringspaces=false,              % don't show spaces in strings
  showtabs=false,                      % don't show tabs in the code
}

\begin{document}

\maketitle

\section*{Question Group 1}
\section*{1.1}
\begin{enumerate}
\item The cumulative distribution function $F(z)$ can be given by: \\
\[
F(z) = \int_{-\infty}^zf(x)dx
\]
Thus we have: \\
\begin{align*}
F(z) &= \int_{-\infty}^0f(x)dx + \int_{0}^{z}f(x)dx \\
F(z) &= 0 + \int_{0}^{z}\lambda \cdot e^{-\lambda \cdot x}dx \\
F(z) &= (-e^{-\lambda \cdot x})_0^z \\
F(z) &= -e^{-\lambda \cdot z} + 1
\end{align*}
\item Given $F(z)$ from the above: \\
\begin{align*}
F(z) &= 0.5 \\
-e^{-\lambda \cdot z} + 1 &= .5 \\
-e^{-\lambda \cdot z} &= -.5 \\
-\lambda \cdot z &= \ln(.5) \\
z &= -\frac{\ln(.5)}{\lambda}
\end{align*}
\end{enumerate}
\section*{1.2}
\begin{enumerate}
\item The z stat for 60 is: \\
\begin{align*}
z &= \frac{60 - 50}{10} \\
z &= 1 \\
\end{align*}
Using a calculator, the cdf of z is .8413
\item we are trying to find the value such that cdf($z$) = .95 where $z$ is the z statistic: \\
\begin{align*}
cdf(z) &= .95 \\
z &= icdf(.95) \\
\frac{x - \mu}{\sigma} &= icdf(.95) \\
x &= icdf(.95) \cdot \sigma + \mu \\
x &\approx 66.4485
\end{align*} 
\end{enumerate}
\section*{Question Group 2}
\section*{2.1}
\begin{enumerate}
\item $\mu$ is a location variable if: \\
\[
f_W(w) = f_Y(w + \mu)
\]
does not depend on $\mu$ where $W = Y - \mu$. \\
For $\xi \neq 0$ we have: \\
\begin{align*}
f_W(w) &= f_Y(w + \mu) \\
&= \frac{1}{\sigma} \cdot (1 + \xi \cdot \frac{(z + \mu) - \mu}{\sigma})^{-1 - \frac{1}{\xi}}\mbox{exp}(-(1 + \xi \cdot \frac{(z + \mu) - \mu}{\sigma})^{-\frac{1}{\xi}}) \\
&= \frac{1}{\sigma} \cdot (1 + \xi \cdot \frac{z}{\sigma})^{-1 - \frac{1}{\xi}}\mbox{exp}(-(1 + \xi \cdot \frac{z}{\sigma})^{-\frac{1}{\xi}}) \\
\end{align*}
The pdf of $f_W(w)$ does not depend on $\mu$ so $\mu$ is a location variable when $\xi \neq 0$ \\
For $\xi = 0$ we have: \\
\begin{align*}
f_W(w) &= f_Y(w + \mu) \\
&= \frac{1}{\sigma} \cdot \mbox{exp}(-\frac{(z + \mu) - \mu}{\sigma})\mbox{exp}(\mbox{-exp}(-\frac{(z + \mu) - \mu}{\sigma})) \\
&= \frac{1}{\sigma} \cdot \mbox{exp}(-\frac{z}{\sigma})\mbox{exp}(\mbox{-exp}(-\frac{z}{\sigma}))
\end{align*}
again the pdf of $f_W(w)$ does not depend on $\mu$ so $\mu$ is a location variable when $\xi = 0$. Therefore $\mu$ is a location variable. \\
$\sigma$ is a scaling variable if: \\
\[
f_W(w) = \sigma \cdot f_Y(\sigma w)
\]
does not depend on $\sigma$ where $W = \frac{Y}{\sigma}$. \\
Since $\mu$ is a location variable, let $Y = Z - \mu$ \\
For $\xi \neq 0$ we have: \\
\begin{align*}
f_W(w) &= \sigma \cdot f_Y(\sigma w) \\
&= \sigma \cdot \frac{1}{\sigma} \cdot (1 + \xi \cdot \frac{y \cdot \sigma}{\sigma})^{-1 - \frac{1}{\xi}}\mbox{exp}(-(1 + \xi \cdot \frac{y \cdot \sigma}{\sigma})^{-\frac{1}{\xi}}) \\
&= (1 + \xi \cdot y)^{-1 - \frac{1}{\xi}}\mbox{exp}(-(1 + \xi \cdot y)^{-\frac{1}{\xi}}) \\
\end{align*}
The final function does not depend on $\sigma$ so $\sigma$ is a scaling variable when $\xi \neq 0$ \\
For $\xi = 0$ we have: \\
\begin{align*}
f_W(w) &= \sigma \cdot f_Y(\sigma w) \\
&= \sigma \cdot \frac{1}{\sigma} \cdot \mbox{exp}(-\frac{y \cdot \sigma}{\sigma})\mbox{exp}(\mbox{-exp}(-\frac{y \cdot \sigma}{\sigma})) \\
&= \mbox{exp}(-y)\mbox{exp}(\mbox{-exp}(-y))
\end{align*}
The final function does not depend on $\sigma$ so $\sigma$ is a scaling variable for $\xi = 0$. $\sigma$ is a scaling variable both when $\xi = 0$ and $\xi \neq 0$ so $\sigma$ is a scaling variable for the family. \\
\item The quantile function is simply the inverse of the cdf: \\
\[
Q(p) = F^{-1}(p)
\]
Thus we have: \\
\begin{align*}
p &= \mbox{exp}(-(1 + \xi(\frac{z - \mu}{\sigma}))^{-\frac{1}{\xi}}) \\
\ln(p) &= -(1 + \xi(\frac{z - \mu}{\sigma}))^{-\frac{1}{\xi}} \\
(-\ln(p))^{-\xi} &= 1 + \xi(\frac{z - \mu}{\sigma}) \\
(-\ln(p))^{-\xi} - 1 &= \xi(\frac{z - \mu}{\sigma}) \\
\frac{(-\ln(p))^{-\xi} - 1}{\xi} \cdot \sigma &= z - \mu \\
z &= \frac{(-\ln(p))^{-\xi} - 1}{\xi} \cdot \sigma + \mu
\end{align*}
Thus the quantile function for $\xi \neq 0$ is: \\
\[
Q(p) = \frac{(-\ln(p))^{-\xi} - 1}{\xi} \cdot \sigma + \mu
\]
for when $\xi = 0$: \\
\begin{align*}
p &= \mbox{exp}(-\mbox{exp}(-\frac{z - \mu}{\sigma})) \\
\ln(p) &= -\mbox{exp}(-\frac{z - \mu}{\sigma}) \\
\ln(-\ln(p)) &= -\frac{z - \mu}{\sigma} \\
-\sigma \cdot \ln(-\ln(p)) + \mu &= z \\
\end{align*}
Thus the quantile function for $\xi = 0$ is: \\
\[
Q(p) = -\sigma \cdot \ln(-\ln(p)) + \mu
\]
\item The probability that a value is greater than $x$ is given by: \\
\[
P(X > x) = 1 - F(x)
\]
Thus we have: \\
\begin{align*}
P(X > 12) &= 1 - F(12) \\
&= 1 - \mbox{exp}(-(1 + \frac{1}{2} \cdot \frac{12 - 10}{2})^{-\frac{1}{\frac{1}{2}}}) \\
&\approx .3588 \\
\end{align*}
\item We simply need to evaluate $Q(.25)$: \\
\begin{align*}
Q(.25) &= \frac{(-\ln(.25))^{-\frac{1}{2}} - 1}{\frac{1}{2}} \cdot 2 + 10 \\
&\approx 9.397
\end{align*}
\end{enumerate}
\section*{2.2}
\begin{enumerate}
\item $\beta$ acts as a scaling parameter if: \\
\[
f_W(w) = \beta \cdot f_Y(\beta w)
\]
does not depend on $\beta$ where $W = \frac{Y}{\beta}$. \\
Thus we have: \\
\begin{align*}
f_W(w) &= \beta \cdot \frac{1}{\beta^{\alpha}\Gamma(\alpha)}(y \cdot \beta)^{\alpha - 1} \cdot e^{\frac{-\beta \cdot y}{\beta}} \\
f_W(w) &= \beta \cdot \frac{1}{\beta \cdot \Gamma(\alpha)}y^{\alpha - 1}\cdot e^{-y} \\
f_W(w) &= \frac{1}{\Gamma(\alpha)}y^{\alpha - 1}\cdot e^{-y} \\
\end{align*}
The final function doesn't rely on $\beta$ so $\beta$ is a scaling variable for $y \geq 0$. The case for $y < 0$ is trivial since the pdf is just 0. So $\beta$ is a scaling variable for this family. \\
\item We now have: \\
\[
f(y) = \frac{1}{\frac{1}{\theta}^{\alpha}\Gamma(\alpha)}(y)^{\alpha - 1} \cdot e^{\frac{-y}{\frac{1}{\theta}}} 
\]
Instead of using $W = \frac{Y}{\theta}$, we will use $W = \frac{Y}{\theta^{-1}}$: \\
\begin{align*}
f_W(w) &= \frac{1}{\theta} \cdot \frac{1}{\frac{1}{\theta}^{\alpha}\Gamma(\alpha)}(y \cdot \theta^{-1})^{\alpha - 1} \cdot e^{\frac{-(y \cdot \theta^{-1})}{\frac{1}{\theta}}} \\
f_W(w) &= \frac{1}{\theta} \cdot \frac{1}{(\theta^{-1})\Gamma(\alpha)}(y^{\alpha - 1}) \cdot e^{-y} \\
f_W(w) &= \frac{1}{\Gamma(\alpha)}(y^{\alpha - 1}) \cdot e^{-y} \\
\end{align*}
The final function doesn't depend on $\theta$ so $\theta$ is a sclaing variable (again $y < 0$ is trivial). 
\end{enumerate}
\section*{2.3}
\begin{enumerate}
\item Assuming the call rate follows a Poisson distribution with $\lambda = 12$ then we have: \\
\[
P(Y = y) = \frac{e^{-12} \cdot 12^y}{y!}
\]
\begin{align*}
P(Y \geq 3) &= 1 - P(Y \leq 2) \\
&= 1 - P(Y = 0) - P(Y = 1) - P(Y = 2) \\
&= 1 - e^{-12} - 12e^{-12} - 72e^{-12} \\
&= 1 - 85 \cdot e^{-12} \\
&= 0.9995 \\
\end{align*}
\item Since the rate of calls is constant, the distribution for the calls in a week also follows a poisson distribution with $\lambda = 12 \cdot 7 = 84$ \\
Thus we have: \\
\[
P(Y = y) = \frac{e^{-84} \cdot 84^y}{y!}
\]
\begin{align*}
P(Y \geq 3) &= 1 - P(Y \leq 2) \\
&= 1 - P(Y = 0) - P(Y = 1) - P(Y = 2) \\
&= 1 - e^{-84} - 84e^{-84} - 3528e^{-84} \\
&\approx 1.0000 \\
\end{align*}
\end{enumerate}
\section*{2.4}
\begin{enumerate}
\item The cdf for an exponential distribution with mean wait time of 10 minutes is given by: \\
\[
F(t) = 1 - e^{-\lambda \cdot t}
\]

\end{enumerate}
\end{document}